backing out the cas stuff ... sticking to upd

ulib/experimental/Steel.Heap.fst
@@ -991,27 +991,25 @@ let upd_action (#a:_) (#pcm:_) (r:ref a pcm)
 let partial_pre_action (fp:slprop u#a) (a:Type u#b) (fp':a -> slprop u#a) =
   hheap fp -> (x:a & hheap (fp' x))
 
-let cas_gen #a (#p:pcm a)
+let upd_gen #a (#p:pcm a)
                (r:ref a p)
                (x v:Ghost.erased a)
-               (f: frame_preserving_cas p x v)
+               (f: frame_preserving_upd p x v)
   : partial_pre_action (pts_to r x)
-                       bool
-                       (fun b -> pts_to r (econd b v x))
+                       unit
+                       (fun _ -> pts_to r v)
   = fun h ->
      let Ref _ _ frac old_v = select_addr h r in
-     match f old_v with
-     | None -> (| false, h |)
-     | Some new_v ->
-       let cell = Ref a p frac new_v in
-       let h' = update_addr h r cell in
-       (| true, h' |)
+     let new_v = f old_v in
+     let cell = Ref a p frac new_v in
+     let h' = update_addr h r cell in
+     (| (), h' |)
 
-let cas_gen_updates_only_r #a (#p:pcm a) (r:ref a p)
+let upd_gen_updates_only_r #a (#p:pcm a) (r:ref a p)
                            (x v:Ghost.erased a)
-                           (f: frame_preserving_cas p x v)
+                           (f: frame_preserving_upd p x v)
                            (h0:hheap (pts_to r x))
-  : Lemma (let (| _, h1 |) = cas_gen r x v f h0 in
+  : Lemma (let (| _, h1 |) = upd_gen r x v f h0 in
            forall s. s <> r ==> h0 s == h1 s)
   = ()
 
@@ -1021,52 +1019,47 @@ let frame_preserving_is_preorder_respecting_pcm_t #a (p:pcm a) (x y:a)
   = PP.frame_preserving_is_preorder_respecting p x y;
     compatible_refl p x
 
-let cas_gen_full_evolution #a (#p:pcm a)
+let upd_gen_full_evolution #a (#p:pcm a)
       (r:ref a p)
       (x y:Ghost.erased a)
-      (f:frame_preserving_cas p x y)
+      (f:frame_preserving_upd p x y)
       (h:full_hheap (pts_to r x))
   : Lemma
     (ensures
-      (let (| _, h1 |) = cas_gen r x y f h in
+      (let (| _, h1 |) = upd_gen r x y f h in
        full_heap_pred h1 /\
        heap_evolves h h1))
   = let old_v = sel_action' r x h in
-    match f old_v with
-    | None -> ()
-    | Some new_v ->
-      assert (frame_preserving p old_v new_v);
-      frame_preserving_is_preorder_respecting_pcm_t p old_v new_v;
-      assert (PP.preorder_of_pcm p old_v new_v);
-      let (| _, h1 |) = cas_gen r x y f h in
-      assert (forall a. a<>r ==> h1 a == h a);
-      assert (forall (x:addr). contains_addr h1 x ==> x==r \/ contains_addr h x);
-      assert (full_heap_pred h1);
-      assert (heap_evolves h h1)
+    let new_v = f old_v in
+    assert (frame_preserving p old_v new_v);
+    frame_preserving_is_preorder_respecting_pcm_t p old_v new_v;
+    assert (PP.preorder_of_pcm p old_v new_v);
+    let (| _, h1 |) = upd_gen r x y f h in
+    assert (forall a. a<>r ==> h1 a == h a);
+    assert (forall (x:addr). contains_addr h1 x ==> x==r \/ contains_addr h x);
+    assert (full_heap_pred h1);
+    assert (heap_evolves h h1)
 
 #push-options "--query_stats --z3rlimit_factor 4"
 
-let cas_gen_frame_preserving #a (#p:pcm a)
+let upd_gen_frame_preserving #a (#p:pcm a)
       (r:ref a p)
       (x y:Ghost.erased a)
-      (f:frame_preserving_cas p x y)
+      (f:frame_preserving_upd p x y)
       (h:hheap (pts_to r x))
       (frame:slprop)
  : Lemma
    (requires interp (pts_to r x `star` frame) h)
    (ensures
-     (let (| b, h1 |) = cas_gen r x y f h in
-      interp (pts_to r (econd b y x) `star` frame) h1 /\
+     (let (| b, h1 |) = upd_gen r x y f h in
+      interp ((pts_to r y) `star` frame) h1 /\
       (forall (hp:hprop frame). hp h == hp h1)))
  = let Ref _ _ frac old_v = select_addr h r in
    let old_v : a = old_v in
-   let (| return_b, h1 |) = cas_gen r x y f h in
-   match f old_v with
-   | None -> ()
-   | Some new_v ->
-     assert (return_b == true);
-     assert (forall a. a<>r ==> h1 a == h a);
-     let aux (hl hr:heap)
+   let (| _, h1 |) = upd_gen r x y f h in
+   let new_v = f old_v in
+   assert (forall a. a<>r ==> h1 a == h a);
+   let aux (hl hr:heap)
        : Lemma
          (requires
            disjoint hl hr /\
@@ -1074,17 +1067,16 @@ let cas_gen_frame_preserving #a (#p:pcm a)
            interp (pts_to r x) hl /\
            interp frame hr)
          (ensures (
-           let (| return_l, hl' |) = cas_gen r x y f hl in
+           let (| _, hl' |) = upd_gen r x y f hl in
            disjoint hl' hr /\
-           h1 == join hl' hr /\
-           return_l == return_b
+           h1 == join hl' hr
            ))
          [SMTPat (disjoint hl hr)]
        = assert (contains_addr hl r);
          let Ref _ _ _ old_v_l = select_addr hl r in
          let old_v_l : a = old_v_l in
-         let (| _, hl' |) = cas_gen r x y f hl in
-         cas_gen_updates_only_r r x y f hl;
+         let (| _, hl' |) = upd_gen r x y f hl in
+         upd_gen_updates_only_r r x y f hl;
          assert (forall s. s<>r ==> hl s == hl' s);
          let Ref _ _ _ new_v_l = select_addr hl' r in
          let new_v_l : a = new_v_l in
@@ -1093,14 +1085,11 @@ let cas_gen_frame_preserving #a (#p:pcm a)
               let old_v_r : a = old_v_r in
               assert (composable p old_v_l old_v_r);
               assert (op p old_v_l old_v_r == old_v); //old_v_l * old_v_r = old_v
-              match f old_v_l with
-              | None -> assert (f old_v == None)
-              | Some new_v_l' ->
-                assert (new_v_l == new_v_l');
-                assert (composable p new_v_l old_v_r);
-                assert (op p new_v_l old_v_r == new_v);
-                assert (disjoint hl' hr);
-                mem_equiv_eq h1 (join hl' hr)
+              assert (new_v_l == f old_v_l);
+              assert (composable p new_v_l old_v_r);
+              assert (op p new_v_l old_v_r == new_v);
+              assert (disjoint hl' hr);
+              mem_equiv_eq h1 (join hl' hr)
          else begin
            assert (old_v_l == old_v);
            assert (new_v == new_v_l);
@@ -1119,23 +1108,7 @@ let cas_gen_frame_preserving #a (#p:pcm a)
      in
      ()
 
-let cas_gen_action #a (#p:pcm a) (r:ref a p) (x y:Ghost.erased a) (f:frame_preserving_cas p x y)
-  : action (pts_to r x)
-           bool
-           (fun b -> pts_to r (econd b y x))
-  = let refined : refined_pre_action
-                    (pts_to r x)
-                    bool
-                    (fun b -> pts_to r (econd b y x))
-     = fun h ->
-         let (|u, h1|) = cas_gen r x y f h in
-         FStar.Classical.forall_intro (FStar.Classical.move_requires (cas_gen_frame_preserving r x y f h));
-         cas_gen_full_evolution #a r x y f h;
-         (| u, h1 |)
-    in
-    refined_pre_action_as_action refined
-
-let upd_gen_action #a (#p:pcm a) (r:ref a p) (x y:Ghost.erased a) (f:frame_preserving_cas p x y{forall x. Some? (f x)})
+let upd_gen_action #a (#p:pcm a) (r:ref a p) (x y:Ghost.erased a) (f:frame_preserving_upd p x y)
   : action (pts_to r x)
            unit
            (fun _ -> pts_to r y)
@@ -1144,9 +1117,9 @@ let upd_gen_action #a (#p:pcm a) (r:ref a p) (x y:Ghost.erased a) (f:frame_prese
                     unit
                     (fun _ -> pts_to r y)
      = fun h ->
-         let (|u, h1|) = cas_gen r x y f h in
-         FStar.Classical.forall_intro (FStar.Classical.move_requires (cas_gen_frame_preserving r x y f h));
-         cas_gen_full_evolution #a r x y f h;
+         let (|u, h1|) = upd_gen r x y f h in
+         FStar.Classical.forall_intro (FStar.Classical.move_requires (upd_gen_frame_preserving r x y f h));
+         upd_gen_full_evolution #a r x y f h;
          (| (), h1 |)
     in
     refined_pre_action_as_action refined
